pulse/lib/pulse/core/PulseCore.Memory.fsti
@@ -16,17 +16,19 @@
 module PulseCore.Memory
 open FStar.Ghost
 open FStar.PCM
-module M_ = PulseCore.NondeterministicMonotonicStateMonad
 module PP = PulseCore.Preorder
 module PST = PulseCore.PreorderStateMonad
 module MSTTotal = PulseCore.MonotonicStateMonad
-/// Building on `PulseCore.Heap`, this module adds memory invariants to the heap to expose the
+module U = FStar.Universe
+module S = FStar.Set
+
+/// This module adds memory invariants to the heap to expose the
 /// final interface for Pulse's PCM-based memory model.
 
 (**** Basic memory properties *)
 
 (** Abstract type of memories *)
-val mem  : Type u#(a + 1)
+val mem  : Type u#(a + 2)
 
 val is_ghost_action (m0 m1:mem u#a) : prop
 let maybe_ghost_action (b:bool) (m0 m1:mem u#a) = b ==> is_ghost_action m0 m1
@@ -47,7 +49,9 @@ val core_mem (m:mem u#a) : mem u#a
 
 (** The type of separation logic propositions. Based on Steel.Heap.slprop *)
 [@@erasable]
-val slprop : Type u#(a + 1)
+val slprop : Type u#(a + 2)
+val is_small (p:slprop u#a) : prop
+let vprop = s:slprop u#a { is_small s }
 
 (** Interpreting mem assertions as memory predicates *)
 val interp (p:slprop u#a) (m:mem u#a) : prop
@@ -60,7 +64,7 @@ val equiv (p1 p2:slprop u#a) : prop
   An extensional equivalence principle for slprop
  *)
 
-val slprop_extensionality (p q:slprop)
+val slprop_extensionality (p q:slprop u#a)
   : Lemma
     (requires p `equiv` q)
     (ensures p == q)
@@ -89,19 +93,18 @@ val core_ref_is_null (r:core_ref) : b:bool { b <==> r == core_ref_null }
 let is_null (#a:Type u#a) (#pcm:pcm a) (r:ref a pcm) : (b:bool{b <==> r == null}) = core_ref_is_null r
 
 (** All the standard connectives of separation logic, based on [Steel.Heap] *)
-val emp : slprop u#a
-val pure (p:prop) : slprop u#a
-val pts_to (#a:Type u#a) (#pcm:_) (r:ref a pcm) (v:a) : slprop u#a
+val emp : vprop u#a
+val pure (p:prop) : vprop u#a
 val star  (p1 p2:slprop u#a) : slprop u#a
 val h_exists (#a:Type u#b) (f: (a -> slprop u#a)) : slprop u#a
 
 (***** Properties of separation logic equivalence *)
 
-val equiv_symmetric (p1 p2:slprop)
-  : squash (p1 `equiv` p2 ==> p2 `equiv` p1)
+// val equiv_symmetric (p1 p2:slprop)
+//   : squash (p1 `equiv` p2 ==> p2 `equiv` p1)
 
-val equiv_extensional_on_star (p1 p2 p3:slprop)
-  : squash (p1 `equiv` p2 ==> (p1 `star` p3) `equiv` (p2 `star` p3))
+// val equiv_extensional_on_star (p1 p2 p3:slprop)
+//   : squash (p1 `equiv` p2 ==> (p1 `star` p3) `equiv` (p2 `star` p3))
 
 val emp_unit (p:slprop)
   : Lemma (p `equiv` (p `star` emp))
@@ -129,9 +132,15 @@ val star_congruence (p1 p2 p3 p4:slprop)
   : Lemma (requires p1 `equiv` p3 /\ p2 `equiv` p4)
           (ensures (p1 `star` p2) `equiv` (p3 `star` p4))
 
-(**** Memory invariants *)
+val small_star_congruence (p1 p2:vprop u#a)
+  : Lemma (is_small (p1 `star` p2))
 
-module S = FStar.Set
+val small_exists_congruence (#a:Type u#a) (p:a -> slprop u#b)
+  : Lemma
+    (requires forall x. is_small (p x))
+    (ensures is_small (h_exists p))
+
+(**** Memory invariants *)
 
 (** Invariants have a name *)
 val iname : eqtype
@@ -157,11 +166,8 @@ let full_mem = m:mem{full_mem_pred m}
 
 (**** Actions *)
 
-/// Note, at this point, using the MSTTotal effect constrains the mem to be
-/// in universe 2, rather than being universe polymorphic
-
 (**
-  The preorder along which the memory evolves with every update. See [Steel.Heap.heap_evolves]
+  The preorder along which the memory evolves with every update.
 *)
 val mem_evolves : FStar.Preorder.preorder full_mem
 
@@ -174,10 +180,10 @@ val mem_evolves : FStar.Preorder.preorder full_mem
 let _MstTot
   (a:Type u#a)
   (except:inames)
-  (expects:slprop u#1)
-  (provides: a -> slprop u#1)
-  (frame:slprop u#1)
-  = MSTTotal.mst #(full_mem u#1) mem_evolves a
+  (expects:slprop u#m)
+  (provides: a -> slprop u#m)
+  (frame:slprop u#m)
+  = MSTTotal.mst #(full_mem u#m) mem_evolves a
     (requires fun m0 ->
         inames_ok except m0 /\
         interp (expects `star` frame `star` locks_invariant except m0) m0)
@@ -190,10 +196,10 @@ let _PST
   (a:Type u#a)
   (maybe_ghost:bool)
   (except:inames)
-  (expects:slprop u#1)
-  (provides: a -> slprop u#1)
-  (frame:slprop u#1)
-= PST.pst #(full_mem u#1) a mem_evolves
+  (expects:slprop u#m)
+  (provides: a -> slprop u#m)
+  (frame:slprop u#m)
+= PST.pst #(full_mem u#m) a mem_evolves
     (requires fun m0 ->
         inames_ok except m0 /\
         interp (expects `star` frame `star` locks_invariant except m0) m0)
@@ -204,8 +210,8 @@ let _PST
         interp (provides x `star` frame `star` locks_invariant except m1) m1)
 
 (** An action is just a thunked computation in [MstTot] that takes a frame as argument *)
-let action_except (a:Type u#a) (except:inames) (expects:slprop) (provides: a -> slprop)
-  : Type u#(max a 2) =
+let action_except (a:Type u#a) (except:inames) (expects:slprop u#um) (provides: a -> slprop u#um)
+  : Type u#(max a (um + 2)) =
   frame:slprop -> _MstTot a except expects provides frame
 
 (** An action is just a thunked computation in [MstTot] that takes a frame as argument *)
@@ -213,120 +219,29 @@ let _pst_action_except
     (a:Type u#a)
     (maybe_ghost:bool)
     (except:inames)
-    (expects:slprop)
-    (provides: a -> slprop)
- : Type u#(max a 2) 
+    (expects:slprop u#um)
+    (provides: a -> slprop u#um)
+ : Type u#(max a (um + 2)) 
  = frame:slprop -> _PST a maybe_ghost except expects provides frame
 
-let pst_action_except (a:Type u#a) (except:inames) (expects:slprop) (provides: a -> slprop) =
+let pst_action_except (a:Type u#a) (except:inames) (expects:slprop u#um) (provides: a -> slprop u#um) =
   _pst_action_except a false except expects provides
 
-let pst_ghost_action_except (a:Type u#a) (except:inames) (expects:slprop) (provides: a -> slprop) =
+let pst_ghost_action_except (a:Type u#a) (except:inames) (expects:slprop u#um) (provides: a -> slprop u#um) =
   _pst_action_except a true except expects provides
 
-val sel_action (#a:Type u#1) (#pcm:_) (e:inames) (r:ref a pcm) (v0:erased a)
-  : pst_action_except (v:a{compatible pcm v0 v}) e (pts_to r v0) (fun _ -> pts_to r v0)
-
-val upd_action (#a:Type u#1) (#pcm:_) (e:inames)
-               (r:ref a pcm)
-               (v0:FStar.Ghost.erased a)
-               (v1:a {FStar.PCM.frame_preserving pcm v0 v1 /\ pcm.refine v1})
-  : pst_action_except unit e (pts_to r v0) (fun _ -> pts_to r v1)
-
-val free_action (#a:Type u#1) (#pcm:pcm a) (e:inames)
-                (r:ref a pcm) (x:FStar.Ghost.erased a{FStar.PCM.exclusive pcm x /\ pcm.refine pcm.FStar.PCM.p.one})
-  : pst_action_except unit e (pts_to r x) (fun _ -> pts_to r pcm.FStar.PCM.p.one)
-
-(** Splitting a permission on a composite resource into two separate permissions *)
-val split_action
-  (#a:Type u#1)
-  (#pcm:pcm a)
-  (e:inames)
-  (r:ref a pcm)
-  (v0:FStar.Ghost.erased a)
-  (v1:FStar.Ghost.erased a{composable pcm v0 v1})
-  : pst_ghost_action_except unit e (pts_to r (v0 `op pcm` v1)) (fun _ -> pts_to r v0 `star` pts_to r v1)
-
-(** Combining separate permissions into a single composite permission *)
-val gather_action
-  (#a:Type u#1)
-  (#pcm:pcm a)
-  (e:inames)
-  (r:ref a pcm)
-  (v0:FStar.Ghost.erased a)
-  (v1:FStar.Ghost.erased a)
-  : pst_ghost_action_except (_:unit{composable pcm v0 v1}) e (pts_to r v0 `star` pts_to r v1) (fun _ -> pts_to r (op pcm v0 v1))
-
-val alloc_action (#a:Type u#1) (#pcm:pcm a) (e:inames) (x:a{pcm.refine x})
-  : pst_action_except (ref a pcm) e emp (fun r -> pts_to r x)
-
-val select_refine (#a:Type u#1) (#p:pcm a)
-                  (e:inames)
-                  (r:ref a p)
-                  (x:erased a)
-                  (f:(v:a{compatible p x v}
-                      -> GTot (y:a{compatible p y v /\
-                                  FStar.PCM.frame_compatible p x v y})))
-  : pst_action_except (v:a{compatible p x v /\ p.refine v}) e
-                      (pts_to r x)
-                      (fun v -> pts_to r (f v))
-
-val upd_gen (#a:Type) (#p:pcm a) (e:inames) (r:ref a p) (x y:Ghost.erased a)
-            (f:FStar.PCM.frame_preserving_upd p x y)
-  : pst_action_except unit e
-                  (pts_to r x)
-                  (fun _ -> pts_to r y)
-
-let property (a:Type)
-  = a -> prop
-
-val witnessed (#a:Type u#1)
-              (#pcm:pcm a)
-              (r:ref a pcm)
-              (fact:property a)
-  : Type0
-
-let stable_property (#a:Type) (pcm:pcm a)
-  = fact:property a {
-       FStar.Preorder.stable fact (PP.preorder_of_pcm pcm)
-    }
-
-val witness (#a:Type) (#pcm:pcm a)
-            (e:inames)
-            (r:erased (ref a pcm))
-            (fact:stable_property pcm)
-            (v:Ghost.erased a)
-            (_:squash (forall z. compatible pcm v z ==> fact z))
-  : action_except (witnessed r fact) e (pts_to r v) (fun _ -> pts_to r v)
-
-val recall (#a:Type u#1) (#pcm:pcm a) (#fact:property a)
-           (e:inames)
-           (r:erased (ref a pcm))
-           (v:Ghost.erased a)
-           (w:witnessed r fact)
-  : action_except (v1:Ghost.erased a{compatible pcm v v1}) e
-                  (pts_to r v)
-                  (fun v1 -> pts_to r v `star` pure (fact v1))
-
-val pts_to_not_null_action 
-      (#a:Type u#1) (#pcm:pcm a)
-      (e:inames)
-      (r:erased (ref a pcm))
-      (v:Ghost.erased a)
-: pst_ghost_action_except (squash (not (is_null r))) e
-    (pts_to r v)
-    (fun _ -> pts_to r v)
 
 (**** Invariants *)
 
 (**[i : inv p] is an invariant whose content is [p] *)
-val pre_inv : Type0
+val pre_inv_aux (p:slprop u#a) : Type0
+let pre_inv : Type0 = pre_inv_aux (emp u#a)
 
-val inv (p:slprop u#1) : Type0
+val inv (p:slprop u#a) : Type0
 
-val pre_inv_of_inv (#p:slprop) (i:inv p) : pre_inv
+val pre_inv_of_inv (#p:slprop u#a) (i:inv p) : pre_inv u#a
 
-val name_of_pre_inv (i:pre_inv) : GTot iname
+val name_of_pre_inv (i:pre_inv u#a) : GTot iname
 
 let name_of_inv (#p:slprop) (i:inv p)
   : GTot iname
@@ -344,20 +259,20 @@ let fresh_wrt (ctx:list pre_inv)
 
 val distinct_invariants_have_distinct_names
       (e:inames)
-      (p:slprop)
-      (q:slprop { p =!= q })
+      (p:slprop u#m)
+      (q:slprop u#m { p =!= q })
       (i:inv p)
       (j:inv q)
-  : action_except (squash (name_of_inv i =!= name_of_inv j)) e emp (fun _ -> emp)
+  : action_except u#0 u#m (squash (name_of_inv i =!= name_of_inv j)) e (emp u#m) (fun _ -> emp u#m)
 
 val invariant_name_identifies_invariant
       (e:inames)
-      (p q:slprop)
+      (p q:slprop u#m)
       (i:inv p)
       (j:inv q { name_of_inv i == name_of_inv j } )
-  : action_except (squash (p == q /\ i == j)) e emp (fun _ -> emp)
+  : action_except (squash (p == q /\ i == j)) e (emp u#m) (fun _ -> emp u#m)
 
-val fresh_invariant (e:inames) (p:slprop) (ctx:list pre_inv)
+val fresh_invariant (e:inames) (p:slprop u#m) (ctx:list (pre_inv u#m))
   : action_except (i:inv p { fresh_wrt ctx (name_of_inv i) }) e p (fun _ -> emp)
 
 val new_invariant (e:inames) (p:slprop)
@@ -372,6 +287,7 @@ val with_invariant (#a:Type)
                    (f:action_except a (add_inv opened_invariants i) (p `star` fp) (fun x -> p `star` fp' x))
   : action_except a opened_invariants fp fp'
 
+(* Some generic actions and combinators *)
 
 val frame (#a:Type)
           (#opened_invariants:inames)
@@ -390,7 +306,6 @@ val pst_frame (#a:Type)
               ($f:_pst_action_except a maybe_ghost opened_invariants pre post)
   : _pst_action_except a maybe_ghost opened_invariants (pre `star` frame) (fun x -> post x `star` frame)
 
-module U = FStar.Universe
 
 val witness_h_exists (#opened_invariants:_) (#a:_) (p:a -> slprop)
   : pst_ghost_action_except (erased a) opened_invariants
@@ -417,6 +332,7 @@ val drop (#opened_invariants:_) (p:slprop)
   : pst_ghost_action_except unit opened_invariants p (fun _ -> emp)
 
 let non_info a = x:erased a -> y:a { reveal x == y}
+
 val lift_ghost
       (#a:Type)
       #opened_invariants #p #q
@@ -424,13 +340,85 @@ val lift_ghost
       (f:erased (pst_ghost_action_except a opened_invariants p q))
   : pst_ghost_action_except a opened_invariants p q
 
+(* Concrete references to "small" types *)
+val pts_to (#a:Type u#a) (#pcm:_) (r:ref a pcm) (v:a) : vprop u#a
+
+val sel_action (#a:Type u#a) (#pcm:_) (e:inames) (r:ref a pcm) (v0:erased a)
+  : pst_action_except (v:a{compatible pcm v0 v}) e (pts_to r v0) (fun _ -> pts_to r v0)
+
+val upd_action (#a:Type u#a) (#pcm:_) (e:inames)
+               (r:ref a pcm)
+               (v0:FStar.Ghost.erased a)
+               (v1:a {FStar.PCM.frame_preserving pcm v0 v1 /\ pcm.refine v1})
+  : pst_action_except unit e (pts_to r v0) (fun _ -> pts_to r v1)
+
+val free_action (#a:Type u#a) (#pcm:pcm a) (e:inames)
+                (r:ref a pcm) (x:FStar.Ghost.erased a{FStar.PCM.exclusive pcm x /\ pcm.refine pcm.FStar.PCM.p.one})
+  : pst_action_except unit e (pts_to r x) (fun _ -> pts_to r pcm.FStar.PCM.p.one)
+
+(** Splitting a permission on a composite resource into two separate permissions *)
+val split_action
+  (#a:Type u#a)
+  (#pcm:pcm a)
+  (e:inames)
+  (r:ref a pcm)
+  (v0:FStar.Ghost.erased a)
+  (v1:FStar.Ghost.erased a{composable pcm v0 v1})
+: pst_ghost_action_except unit e
+    (pts_to r (v0 `op pcm` v1))
+    (fun _ -> pts_to r v0 `star` pts_to r v1)
+
+(** Combining separate permissions into a single composite permission *)
+val gather_action
+  (#a:Type u#a)
+  (#pcm:pcm a)
+  (e:inames)
+  (r:ref a pcm)
+  (v0:FStar.Ghost.erased a)
+  (v1:FStar.Ghost.erased a)
+: pst_ghost_action_except (squash (composable pcm v0 v1)) e
+    (pts_to r v0 `star` pts_to r v1)
+    (fun _ -> pts_to r (op pcm v0 v1))
+
+val alloc_action (#a:Type u#a) (#pcm:pcm a) (e:inames) (x:a{pcm.refine x})
+: pst_action_except (ref a pcm) e
+    emp
+    (fun r -> pts_to r x)
+
+val select_refine (#a:Type u#a) (#p:pcm a)
+                  (e:inames)
+                  (r:ref a p)
+                  (x:erased a)
+                  (f:(v:a{compatible p x v}
+                      -> GTot (y:a{compatible p y v /\
+                                  FStar.PCM.frame_compatible p x v y})))
+: pst_action_except (v:a{compatible p x v /\ p.refine v}) e
+    (pts_to r x)
+    (fun v -> pts_to r (f v))
+
+val upd_gen (#a:Type u#a) (#p:pcm a) (e:inames) (r:ref a p) (x y:Ghost.erased a)
+            (f:FStar.PCM.frame_preserving_upd p x y)
+: pst_action_except unit e
+    (pts_to r x)
+    (fun _ -> pts_to r y)
+
+val pts_to_not_null_action 
+      (#a:Type u#a) (#pcm:pcm a)
+      (e:inames)
+      (r:erased (ref a pcm))
+      (v:Ghost.erased a)
+: pst_ghost_action_except (squash (not (is_null r))) e
+    (pts_to r v)
+    (fun _ -> pts_to r v)
+
+(* Ghost references to "small" types *)
 [@@erasable]
 val ghost_ref (#[@@@unused] a:Type u#a) ([@@@unused]p:pcm a) : Type0
-val ghost_pts_to (#a:Type u#a) (#p:pcm a) (r:ghost_ref p) (v:a) : slprop u#a
+val ghost_pts_to (#a:Type u#a) (#p:pcm a) (r:ghost_ref p) (v:a) : vprop u#a
 
 val ghost_alloc
     (#o:_)
-    (#a:Type u#1)
+    (#a:Type u#a)
     (#pcm:pcm a)
     (x:erased a{pcm.refine x})
 : pst_ghost_action_except
@@ -487,3 +475,166 @@ val ghost_gather
     (squash (composable pcm v0 v1)) o
     (ghost_pts_to r v0 `star` ghost_pts_to r v1)
     (fun _ -> ghost_pts_to r (op pcm v0 v1))
+
+(* Concrete references to "big" types *)
+val big_pts_to (#a:Type u#(a + 1)) (#pcm:_) (r:ref a pcm) (v:a) : slprop u#a
+
+val big_sel_action
+      (#a:Type u#(a + 1))
+      (#pcm:_)
+      (e:inames)
+      (r:ref a pcm)
+      (v0:erased a)
+: pst_action_except (v:a{compatible pcm v0 v}) e
+    (big_pts_to r v0)
+    (fun _ -> big_pts_to r v0)
+
+val big_upd_action
+      (#a:Type u#(a + 1)) (#pcm:_) (e:inames)
+      (r:ref a pcm)
+      (v0:FStar.Ghost.erased a)
+      (v1:a {FStar.PCM.frame_preserving pcm v0 v1 /\ pcm.refine v1})
+: pst_action_except unit e
+    (big_pts_to r v0)
+    (fun _ -> big_pts_to r v1)
+
+val big_free_action
+      (#a:Type u#(a + 1))
+      (#pcm:pcm a)
+      (e:inames)
+      (r:ref a pcm)
+      (x:FStar.Ghost.erased a{FStar.PCM.exclusive pcm x /\ pcm.refine pcm.FStar.PCM.p.one})
+: pst_action_except unit e
+    (big_pts_to r x)
+    (fun _ -> big_pts_to r pcm.FStar.PCM.p.one)
+
+(** Splitting a permission on a composite resource into two separate permissions *)
+val big_split_action
+      (#a:Type u#(a + 1))
+      (#pcm:pcm a)
+      (e:inames)
+      (r:ref a pcm)
+      (v0:FStar.Ghost.erased a)
+      (v1:FStar.Ghost.erased a{composable pcm v0 v1})
+: pst_ghost_action_except unit e
+    (big_pts_to r (v0 `op pcm` v1))
+    (fun _ -> big_pts_to r v0 `star` big_pts_to r v1)
+
+(** Combining separate permissions into a single composite permission *)
+val big_gather_action
+      (#a:Type u#(a + 1))
+      (#pcm:pcm a)
+      (e:inames)
+      (r:ref a pcm)
+      (v0:FStar.Ghost.erased a)
+      (v1:FStar.Ghost.erased a)
+: pst_ghost_action_except (squash (composable pcm v0 v1)) e
+    (big_pts_to r v0 `star` big_pts_to r v1)
+    (fun _ -> big_pts_to r (op pcm v0 v1))
+
+val big_alloc_action
+      (#a:Type u#(a + 1))
+      (#pcm:pcm a)
+      (e:inames)
+      (x:a{pcm.refine x})
+: pst_action_except (ref a pcm) e
+    emp
+    (fun r -> big_pts_to r x)
+
+val big_select_refine
+      (#a:Type u#(a + 1))
+      (#p:pcm a)
+      (e:inames)
+      (r:ref a p)
+      (x:erased a)
+      (f:(v:a{compatible p x v}
+          -> GTot (y:a{compatible p y v /\
+                      FStar.PCM.frame_compatible p x v y})))
+: pst_action_except (v:a{compatible p x v /\ p.refine v}) e
+    (big_pts_to r x)
+    (fun v -> big_pts_to r (f v))
+
+val big_upd_gen
+    (#a:Type u#(a + 1))
+    (#p:pcm a)
+    (e:inames)
+    (r:ref a p)
+    (x y:Ghost.erased a)
+    (f:FStar.PCM.frame_preserving_upd p x y)
+: pst_action_except unit e
+    (big_pts_to r x)
+    (fun _ -> big_pts_to r y)
+
+val big_pts_to_not_null_action 
+      (#a:Type u#(a + 1))
+      (#pcm:pcm a)
+      (e:inames)
+      (r:erased (ref a pcm))
+      (v:Ghost.erased a)
+: pst_ghost_action_except (squash (not (is_null r))) e
+    (big_pts_to r v)
+    (fun _ -> big_pts_to r v)
+
+(* Ghost references to "small" types *)
+val big_ghost_pts_to (#a:Type u#(a + 1)) (#p:pcm a) (r:ghost_ref p) (v:a) : slprop u#a
+
+val big_ghost_alloc
+    (#o:_)
+    (#a:Type u#(a + 1))
+    (#pcm:pcm a)
+    (x:erased a{pcm.refine x})
+: pst_ghost_action_except
+    (ghost_ref pcm)
+    o
+    emp 
+    (fun r -> big_ghost_pts_to r x)
+
+val big_ghost_read
+    #o
+    (#a:Type u#(a + 1))
+    (#p:pcm a)
+    (r:ghost_ref p)
+    (x:erased a)
+    (f:(v:a{compatible p x v}
+        -> GTot (y:a{compatible p y v /\
+                     FStar.PCM.frame_compatible p x v y})))
+: pst_ghost_action_except
+    (erased (v:a{compatible p x v /\ p.refine v}))
+    o
+    (big_ghost_pts_to r x)
+    (fun v -> big_ghost_pts_to r (f v))
+
+val big_ghost_write
+    #o
+    (#a:Type u#(a + 1))
+    (#p:pcm a)
+    (r:ghost_ref p)
+    (x y:Ghost.erased a)
+    (f:FStar.PCM.frame_preserving_upd p x y)
+: pst_ghost_action_except unit o 
+    (big_ghost_pts_to r x)
+    (fun _ -> big_ghost_pts_to r y)
+
+val big_ghost_share
+    #o
+    (#a:Type u#(a + 1))
+    (#pcm:pcm a)
+    (r:ghost_ref pcm)
+    (v0:FStar.Ghost.erased a)
+    (v1:FStar.Ghost.erased a{composable pcm v0 v1})
+: pst_ghost_action_except unit o
+    (big_ghost_pts_to r (v0 `op pcm` v1))
+    (fun _ -> big_ghost_pts_to r v0 `star` big_ghost_pts_to r v1)
+
+val big_ghost_gather
+    #o
+    (#a:Type u#(a + 1))
+    (#pcm:pcm a)
+    (r:ghost_ref pcm)
+    (v0:FStar.Ghost.erased a)
+    (v1:FStar.Ghost.erased a)
+: pst_ghost_action_except
+    (squash (composable pcm v0 v1)) o
+    (big_ghost_pts_to r v0 `star` big_ghost_pts_to r v1)
+    (fun _ -> big_ghost_pts_to r (op pcm v0 v1))
+
